src/Pipit.Sugar.fst
@@ -17,28 +17,63 @@ module S = Pipit.Sugar.Base
 
 module R = FStar.Real
 
-type s (t: valtype) = S.s table t
-type bools = s TBool
-type ints = s TInt
-type reals = s TReal
+type valtype' (a: Type) = v: valtype { ty_sem v == a }
+type arithtype' (a: Type) = v: arithtype { ty_sem v == a }
 
-let run (#a: valtype) (e: s a) : val_exp table [] a = S.run e
-let run1 (#a #b: valtype) (f: s a -> s b) : val_exp table [a] b = S.run1 f
-let run2 (#a #b #c: valtype) (f: s a -> s b -> s c) : val_exp table [a; b] c = S.run2 f
+class is_valtype (a: Type) = {
+  is_valtype_get: valtype' a;
+}
 
-let pure (#t: valtype) (v: table.ty_sem t): s t = S.pure v
+instance is_valtype_bool: is_valtype bool = {
+  is_valtype_get = TBool;
+}
+instance is_valtype_int: is_valtype int = {
+  is_valtype_get = TInt;
+}
+instance is_valtype_real: is_valtype R.real = {
+  is_valtype_get = TReal;
+}
+instance is_valtype_pair {| is_valtype 'a |} {| is_valtype 'b |}: is_valtype ('a & 'b) = {
+  is_valtype_get = TPair (is_valtype_get #'a) (is_valtype_get #'b);
+}
+
+class is_arithtype (a: Type) = {
+  // is_arithtype_valtype: is_valtype a;
+  is_arithtype_get: arithtype' a;
+}
+instance is_arithtype_int: is_arithtype int = {
+  // is_arithtype_valtype = {| is_valtype int |};
+  is_arithtype_get = TInt;
+}
+instance is_arithtype_real: is_arithtype R.real = {
+  is_arithtype_get = TReal;
+}
+
+// type s  (a: valtype)  = S.s table a
+type s (a: Type) = S.s' table a
+
+type bools = s bool
+type ints  = s int
+type reals = s R.real
+
+let run  (e: s 'a) : exp table [] 'a = S.run e
+
+let run1 {| is_valtype 'a |} (f: s 'a -> s 'b) : exp table [is_valtype_get #'a ] 'b = S.run1 f
+let run2 {| is_valtype 'a |} {| is_valtype 'b |} (f: s 'a -> s 'b -> s 'c) : exp table [is_valtype_get #'a; is_valtype_get #'b] 'c = S.run2 f
+
+let pure {| is_valtype 'a |} (v: 'a): s 'a = S.pure #table #(is_valtype_get #'a) v
 
 // LATER: explicit let' should not be necessary once we have CSE / sharing recovery
-let let' (#a #b: valtype) (e: s a) (f: s a -> s b) = S.let' e f
+let let' {| is_valtype 'a |} {| is_valtype 'b |} (e: s 'a) (f: s 'a -> s 'b) = S.let' #table #(is_valtype_get #'a) #(is_valtype_get #'b) e f
 
-let rec' (#a: valtype) (f: s a -> s a): s a = S.rec' f
+let rec' {| is_valtype 'a |} (f: s 'a -> s 'a): s 'a = S.rec' #table #(is_valtype_get #'a) f
 
-let check' (#a: valtype) (name: string) (e: bools) (f: s a): s a =
-  S.check' name e f
+let check' {| is_valtype 'a |} (name: string) (e: bools) (f: s 'a): s 'a =
+  S.check' #table #(is_valtype_get #'a) name e f
 
-let fby (#a: valtype) (v: ty_sem a) (e: s a): s a = S.fby v e
-let pre (#a: valtype) (e: s a): s a = S.pre e
-let (-->) (#a: valtype) (e1 e2: s a): s a = S.(e1 --> e2)
+let fby {| is_valtype 'a |} (v: 'a) (e: s 'a): s 'a = S.fby #table #(is_valtype_get #'a) v e
+let pre {| is_valtype 'a |} (e: s 'a): s 'a = S.pre #table #(is_valtype_get #'a) e
+let (-->) {| is_valtype 'a |} (e1 e2: s 'a): s 'a = S.((-->) #table #(is_valtype_get #'a) e1 e2)
 
 
 let tt: bools = pure true
@@ -48,9 +83,9 @@ let z (i: int): ints = S.pure i
 let z0 = z 0
 let z1 = z 1
 
-let zero (#t: arithtype): s t = match t with
+let zero {| is_arithtype 'a |}: s 'a = match is_arithtype_get #'a with
  | TInt  -> z0
- | TReal -> pure R.zero
+ | TReal -> S.pure #table #(is_arithtype_get #'a) R.zero
 
 (* Working with booleans *)
 let (/\): bools -> bools -> bools = S.liftP2 (P'B P'B'And)
@@ -62,18 +97,31 @@ let (!^) = op_Negation
 let not_ = op_Negation
 
 (* Arithmetic operators, "^" suffix means "lifted" but unfortunately boolean operators such as /\^ do not parse *)
-let (=^) (#t: valtype): s t -> s t -> bools = S.liftP2 (P'V P'V'Eq t)
-let (<>^) (#t: valtype): s t -> s t -> bools = S.liftP2 (P'V P'V'Ne t)
+let (=^) {| is_valtype 'a |}: s 'a -> s 'a -> bools =
+  S.liftP2 #table #(is_valtype_get #'a) #(is_valtype_get #'a) (P'V P'V'Eq (is_valtype_get #'a))
+let (<>^) {| is_valtype 'a |}: s 'a -> s 'a -> bools =
+  S.liftP2 #table #(is_valtype_get #'a) #(is_valtype_get #'a) (P'V P'V'Ne (is_valtype_get #'a))
 
-let (+^) (#t: arithtype): s t -> s t -> s t = S.liftP2 (P'A P'A'Add t)
-let (-^) (#t: arithtype): s t -> s t -> s t = S.liftP2 (P'A P'A'Sub t)
-let (/^) (#t: arithtype): s t -> s t -> s t = S.liftP2 (P'A P'A'Div t)
-let ( *^ ) (#t: arithtype): s t -> s t -> s t = S.liftP2 (P'A P'A'Mul t)
+let (+^) {| is_arithtype 'a |}: s 'a -> s 'a -> s 'a =
+  S.liftP2 #table #(is_arithtype_get #'a) #(is_arithtype_get #'a) #(is_arithtype_get #'a) (P'A P'A'Add (is_arithtype_get #'a))
+let (-^) {| is_arithtype 'a |}: s 'a -> s 'a -> s 'a =
+  S.liftP2 #table #(is_arithtype_get #'a) #(is_arithtype_get #'a) #(is_arithtype_get #'a) (P'A P'A'Sub (is_arithtype_get #'a))
+let (/^) {| is_arithtype 'a |}: s 'a -> s 'a -> s 'a =
+  S.liftP2 #table #(is_arithtype_get #'a) #(is_arithtype_get #'a) #(is_arithtype_get #'a) (P'A P'A'Div (is_arithtype_get #'a))
+let ( *^ ) {| is_arithtype 'a |}: s 'a -> s 'a -> s 'a =
+  S.liftP2 #table #(is_arithtype_get #'a) #(is_arithtype_get #'a) #(is_arithtype_get #'a) (P'A P'A'Mul (is_arithtype_get #'a))
 
-let (<=^) (#t: arithtype): s t -> s t -> bools = S.liftP2 (P'A P'A'Le t)
-let (<^) (#t: arithtype): s t -> s t -> bools = S.liftP2 (P'A P'A'Lt t)
-let (>=^) (#t: arithtype): s t -> s t -> bools = S.liftP2 (P'A P'A'Ge t)
-let (>^) (#t: arithtype): s t -> s t -> bools = S.liftP2 (P'A P'A'Gt t)
+let (<=^) {| is_arithtype 'a |}: s 'a -> s 'a -> bools =
+  S.liftP2 #table #(is_arithtype_get #'a) #(is_arithtype_get #'a) (P'A P'A'Le (is_arithtype_get #'a))
+let (<^) {| is_arithtype 'a |}: s 'a -> s 'a -> bools =
+  S.liftP2 #table #(is_arithtype_get #'a) #(is_arithtype_get #'a) (P'A P'A'Lt (is_arithtype_get #'a))
+let (>=^) {| is_arithtype 'a |}: s 'a -> s 'a -> bools =
+  S.liftP2 #table #(is_arithtype_get #'a) #(is_arithtype_get #'a) (P'A P'A'Ge (is_arithtype_get #'a))
+let (>^) {| is_arithtype 'a |}: s 'a -> s 'a -> bools =
+  S.liftP2 #table #(is_arithtype_get #'a) #(is_arithtype_get #'a) (P'A P'A'Gt (is_arithtype_get #'a))
+
+let tup {| is_valtype 'a |} {| is_valtype 'b |}: s 'a -> s 'b -> s ('a & 'b) =
+  S.liftP2 #table #(is_valtype_get #'a) #(is_valtype_get #'b) #(TPair (is_valtype_get #'a) (is_valtype_get #'b)) (P'T P'T'Pair (is_valtype_get #'a) (is_valtype_get #'b))
 
 let tup (#a #b: valtype): s a -> s b -> s (TPair a b) = S.liftP2 (P'T P'T'Pair a b)
 let fst (#a #b: valtype): s (TPair a b) -> s a = S.liftP1 (P'T P'T'Fst a b)
